theories/rlist.v
@@ -1,185 +1,142 @@
-From stdpp Require Export option.
-Require Export base.
-From stdpp Require Import list.
-
-Export Nat Lia.
+From stdpp Require Export decidable.
+From stdpp Require Import numbers.
 
 
-(** ** Reverse list interface *)
+Record rlist (A : Type) : Type := {
+  rl_length :> nat;
+  rl_map :> nat -> A
+}.
+Arguments Build_rlist {A}.
+Arguments rl_length {A}.
+Arguments rl_map {A}.
 
-Module Type RLIST.
-  Parameter rlist : Type -> Type.
-
-  Parameter rlength : forall {A}, rlist A -> nat.
-
-  Declare Instance rlist_lookup {A} : Lookup nat A (rlist A).
-
-  Axiom is_Some_lookup : forall {A} (c : rlist A) n,
-    is_Some (c !! n) <-> n < rlength c.
-
-  (** Build a list from its length and its (total) lookup function *)
-  Parameter build_rlist : forall {A}, nat -> (nat -> A) -> rlist A.
-
-  Axiom rlength_build_rlist : forall {A} n (f : nat -> A),
-    rlength (build_rlist n f) = n.
-  Axiom lookup_build_rlist : forall {A} l (f : nat -> A) n,
-    n < l -> build_rlist l f !! n = Some (f n).
-
-  Declare Instance rlist_fmap : FMap rlist.
-
-  Axiom lookup_fmap : forall {A} {B} (f : A -> B) (l : rlist A) n,
-    (f <$> l) !! n = f <$> l !! n.
-End RLIST.
+Declare Scope rlist_scope.
+Delimit Scope rlist_scope with rlist.
+Open Scope rlist_scope.
 
 
-(** ** Reverse list theories *)
+Definition lookup_default {A} d n (l : rlist A) : A :=
+  if decide (n < l) then l n else d.
 
-Module RlistTheories (Rlist : RLIST).
-  Export Rlist.
+Definition rl_cons {A} (l : rlist A) a :=
+  Build_rlist (S l) (fun n => if decide (n < l) then l n else a).
 
-  Notation "|( c )|" := (rlength c) : stlc_scope.
+Notation "l +: e" := (rl_cons l e) (at level 50) : rlist_scope.
 
+Instance rlist_fmap : FMap rlist :=
+  fun _ _ f l => Build_rlist l (fun n => f (l n)).
 
-  Definition lookup_default {A} d n (c : rlist A) : A :=
-    match c !! n with
-    | None => d
-    | Some x => x
-    end.
+(*
+Theorem rlength_rcons : forall {A} (c : rlist A) t,
+  rlength (rcons c t) = S (rlength c).
+Proof.
+  intros. unfold rcons. apply rlength_build_rlist.
+Qed.
 
-  Theorem lookup_None1 {A} (c : rlist A) n :
-    n >= |(c)| -> c !! n = None.
-  Proof.
-    intros H.
-    destruct (c !! n) eqn : E; [|reflexivity].
-    assert (n < |(c)|); [|lia].
-    apply is_Some_lookup.
-    econstructor. eassumption.
-  Qed.
+Theorem lookup_rcons_eq : forall {A} (c : rlist A) t n,
+  n = rlength c -> rcons c t !! n = Some t.
+Proof.
+  intros.
+  unfold rcons. rewrite lookup_build_rlist; [|lia].
+  f_equal. rewrite decide_False; [easy|lia].
+Qed.
 
-  Theorem lookup_None2 {A} (c : rlist A) n :
-    c !! n = None -> n >= |(c)|.
-  Proof.
-    intros H.
-    destruct (decide (n < |(c)|)); [|lia].
-    apply is_Some_lookup in l. destruct l. now rewrite H in H0.
-  Qed.
+Theorem lookup_rcons_lt : forall {A} (c : rlist A) t n,
+  n < rlength c -> (c +: t) !! n = c !! n.
+Proof.
+  intros * H.
+  unfold rcons. rewrite lookup_build_rlist; [|lia].
+  apply is_Some_lookup in H as Hx. destruct Hx as [x Hx]. rewrite Hx.
+  f_equal. rewrite decide_True; [|easy].
+  unfold lookup_default. now rewrite Hx.
+Qed.
 
+Theorem lookup_rcons_gt : forall {A} (c : rlist A) t n,
+  n > |(c)| -> rcons c t !! n = None.
+Proof.
+  intros. apply lookup_None1.
+  rewrite rlength_rcons. lia.
+Qed.
 
-  Definition rcons {A} (l : rlist A) a :=
-    build_rlist (S |(l)|) (fun n => if decide (n < |(l)|) then lookup_default a n l else a).
+Inductive lookup_rcons_cases {A} (c : rlist A) t n : Prop :=
+  | lookup_rcons_cases_lt (_ : n < |(c)|) (_ : (c +: t) !! n = c !! n)
+  | lookup_rcons_cases_eq (_ : n = |(c)|) (_ : (c +: t) !! n = Some t)
+  | lookup_rcons_cases_gt (_ : n > |(c)|) (_ : (c +: t) !! n = None).
 
-  Notation "l +: e" := (rcons l e) (at level 50) : stlc_scope.
+Theorem lookup_rcons_spec {A} (c : rlist A) t n : lookup_rcons_cases c t n.
+Proof.
+  destruct (lt_total n |(c)|) as [H | [H | H]].
+  - apply lookup_rcons_cases_lt; [assumption|].
+    now apply lookup_rcons_lt.
+  - apply lookup_rcons_cases_eq; [assumption|].
+    now apply lookup_rcons_eq.
+  - apply lookup_rcons_cases_gt; [assumption|].
+    now apply lookup_rcons_gt.
+Qed.
 
-  Theorem rlength_rcons : forall {A} (c : rlist A) t,
-    rlength (rcons c t) = S (rlength c).
-  Proof.
-    intros. unfold rcons. apply rlength_build_rlist.
-  Qed.
+Ltac lookup_rcons_spec c t n H E :=
+  destruct (lookup_rcons_spec c t n) as [H E | H E | H E]; rewrite E in *.
 
-  Theorem lookup_rcons_eq : forall {A} (c : rlist A) t n,
-    n = rlength c -> rcons c t !! n = Some t.
-  Proof.
-    intros.
-    unfold rcons. rewrite lookup_build_rlist; [|lia].
-    f_equal. rewrite decide_False; [easy|lia].
-  Qed.
+Theorem is_Some_rlength {A B} (l : rlist A) (h : rlist B) :
+  (forall n, is_Some (l !! n) <-> is_Some (h !! n)) ->
+  |(l)| = |(h)|.
+Proof.
+  intros H. destruct (lt_total |(l)| |(h)|) as [E|[L|G]]; try assumption.
+  - apply is_Some_lookup in E. apply H in E.
+    apply is_Some_lookup in E. lia.
+  - apply is_Some_lookup in G. apply H in G.
+    apply is_Some_lookup in G. lia.
+Qed.
 
-  Theorem lookup_rcons_lt : forall {A} (c : rlist A) t n,
-    n < rlength c -> (c +: t) !! n = c !! n.
-  Proof.
-    intros * H.
-    unfold rcons. rewrite lookup_build_rlist; [|lia].
-    apply is_Some_lookup in H as Hx. destruct Hx as [x Hx]. rewrite Hx.
-    f_equal. rewrite decide_True; [|easy].
-    unfold lookup_default. now rewrite Hx.
-  Qed.
-
-  Theorem lookup_rcons_gt : forall {A} (c : rlist A) t n,
-    n > |(c)| -> rcons c t !! n = None.
-  Proof.
-    intros. apply lookup_None1.
-    rewrite rlength_rcons. lia.
-  Qed.
-
-  Inductive lookup_rcons_cases {A} (c : rlist A) t n : Prop :=
-    | lookup_rcons_cases_lt (_ : n < |(c)|) (_ : (c +: t) !! n = c !! n)
-    | lookup_rcons_cases_eq (_ : n = |(c)|) (_ : (c +: t) !! n = Some t)
-    | lookup_rcons_cases_gt (_ : n > |(c)|) (_ : (c +: t) !! n = None).
-
-  Theorem lookup_rcons_spec {A} (c : rlist A) t n : lookup_rcons_cases c t n.
-  Proof.
-    destruct (lt_total n |(c)|) as [H | [H | H]].
-    - apply lookup_rcons_cases_lt; [assumption|].
-      now apply lookup_rcons_lt.
-    - apply lookup_rcons_cases_eq; [assumption|].
-      now apply lookup_rcons_eq.
-    - apply lookup_rcons_cases_gt; [assumption|].
-      now apply lookup_rcons_gt.
-  Qed.
-
-  Ltac lookup_rcons_spec c t n H E :=
-    destruct (lookup_rcons_spec c t n) as [H E | H E | H E]; rewrite E in *.
-
-  Theorem is_Some_rlength {A B} (l : rlist A) (h : rlist B) :
-    (forall n, is_Some (l !! n) <-> is_Some (h !! n)) ->
-    |(l)| = |(h)|.
-  Proof.
-    intros H. destruct (lt_total |(l)| |(h)|) as [E|[L|G]]; try assumption.
-    - apply is_Some_lookup in E. apply H in E.
-      apply is_Some_lookup in E. lia.
-    - apply is_Some_lookup in G. apply H in G.
-      apply is_Some_lookup in G. lia.
-  Qed.
-
-  Theorem rlength_fmap : forall {A} {B} (f : A -> B) l,
-    |(f <$> l)| = |(l)|.
-  Proof.
-    intros. apply is_Some_rlength.
-    intros. rewrite lookup_fmap. apply fmap_is_Some.
-  Qed.
+Theorem rlength_fmap : forall {A} {B} (f : A -> B) l,
+  |(f <$> l)| = |(l)|.
+Proof.
+  intros. apply is_Some_rlength.
+  intros. rewrite lookup_fmap. apply fmap_is_Some.
+Qed.
 End RlistTheories.
 
 
 (** ** Reverse list implementation *)
 
 Module RlistList <: RLIST.
-  Definition rlist := list.
-  Definition rlength := @length.
+Definition rlist := list.
+Definition rlength := @length.
 
-  Instance rlist_lookup {A} : Lookup nat A (rlist A) := list_lookup.
+Instance rlist_lookup {A} : Lookup nat A (rlist A) := list_lookup.
 
-  Theorem is_Some_lookup {A} :
-    forall (c : rlist A) n, is_Some (c !! n) <-> n < length c.
-  Proof. apply lookup_lt_is_Some. Qed.
+Theorem is_Some_lookup {A} :
+  forall (c : rlist A) n, is_Some (c !! n) <-> n < length c.
+Proof. apply lookup_lt_is_Some. Qed.
 
-  Fixpoint build_rlist {A} n f : rlist A :=
-    match n with
-    | 0 => []
-    | S n => build_rlist n f ++ [f n]
-    end.
+Fixpoint build_rlist {A} n f : rlist A :=
+  match n with
+  | 0 => []
+  | S n => build_rlist n f ++ [f n]
+  end.
 
-  Theorem rlength_build_rlist : forall {A} n (f : nat -> A),
-    length (build_rlist n f) = n.
-  Proof.
-    intros. induction n; [reflexivity|].
-    simpl. rewrite length_app. rewrite IHn. simpl. lia.
-  Qed.
+Theorem rlength_build_rlist : forall {A} n (f : nat -> A),
+  length (build_rlist n f) = n.
+Proof.
+  intros. induction n; [reflexivity|].
+  simpl. rewrite length_app. rewrite IHn. simpl. lia.
+Qed.
 
-  Theorem lookup_build_rlist : forall {A} n (f : nat -> A) x,
-    x < n -> build_rlist n f !! x = Some (f x).
-  Proof.
-    intros. induction n; [lia|].
-    simpl. destruct (decide (x = n)).
-    - subst. rewrite @lookup_app_r; rewrite rlength_build_rlist; [|lia].
-      now rewrite sub_diag.
-    - rewrite @lookup_app_l.
-      + apply IHn. lia.
-      + rewrite rlength_build_rlist. lia.
-  Qed.
+Theorem lookup_build_rlist : forall {A} n (f : nat -> A) x,
+  x < n -> build_rlist n f !! x = Some (f x).
+Proof.
+  intros. induction n; [lia|].
+  simpl. destruct (decide (x = n)).
+  - subst. rewrite @lookup_app_r; rewrite rlength_build_rlist; [|lia].
+    now rewrite sub_diag.
+  - rewrite @lookup_app_l.
+    + apply IHn. lia.
+    + rewrite rlength_build_rlist. lia.
+Qed.
 
-  Instance rlist_fmap : FMap rlist := list_fmap.
+Instance rlist_fmap : FMap rlist := list_fmap.
 
-  Theorem lookup_fmap : forall {A} {B} (f : A -> B) (l : rlist A) n,
-    (f <$> l) !! n = f <$> l !! n.
-  Proof. intros. apply list_lookup_fmap. Qed.
-End RlistList.
+Theorem lookup_fmap : forall {A} {B} (f : A -> B) (l : rlist A) n,
+  (f <$> l) !! n = f <$> l !! n.
+Proof. intros. apply list_lookup_fmap. Qed.
+*)
