theories/glogic.v
@@ -1,5 +1,6 @@
-From stdpp Require Import list sets.
-Require Import g_stlc.
+Require Export g_stlc.
+From stdpp Require Import sets.
+Close Scope list_scope.
 
 
 (*************************)
@@ -42,8 +43,7 @@ Module GLogic (SqSet : SQ_SET).
 
   Inductive is_derivable : sequent -> Prop :=
     | rl_id C a b :
-        has_type C a ty_prp ->
-        tm_equiv |(C)| a b ->
+        has_type C a ty_prp -> tm_equiv C a b ->
         is_derivable (sq_build C {[a]} b)
     | rl_cut C l m b c :
         is_derivable (sq_build C l b) ->
@@ -94,45 +94,61 @@ Module GLogic (SqSet : SQ_SET).
         is_derivable (sq_build C l <{ b > c }>)
     | rl_forL C T l b c t :
         has_type C t T ->
-        is_derivable (sq_build C (subst_last |(C)| t b :: l) c) ->
+        is_derivable (sq_build C (subst_last C C t b :: l) c) ->
         is_derivable (sq_build C (<{for T, b}> :: l) c)
     | rl_forR C T l b sb :
-        (forall t, t ∈ sb <-> t ∈ supp b) ->
-        is_derivable (sq_build (C +: foldr ty_arr T (has_type_other <$> sb)) (sq_set_map (bound_level_map S |(C)|) l) (
-          subst_last2 (S |(C)|) |(C)| (foldl tm_app (tm_lvl |(C)|) sb) b
+        (forall t, t ∈ sb <-> in_supp b t) ->
+        is_derivable (sq_build (C +: foldr ty_arr T (type_check_other <$> sb)) (sq_set_map (lift C) l) (
+          subst_last C (S C) (foldl tm_app (tm_lvl C) sb) b
         )) ->
         is_derivable (sq_build C l <{for T, b}>)
     | rl_exL C T l b c sb :
-        (forall t, t ∈ sb <-> t ∈ supp b) ->
-        is_derivable (sq_build (C +: foldr ty_arr T (has_type_other <$> sb)) ((
-          subst_last2 (S |(C)|) |(C)| (foldl tm_app (tm_lvl |(C)|) sb) b
-        ) :: (sq_set_map (bound_level_map S |(C)|) l)) (bound_level_map S |(C)| c)) ->
+        (forall t, t ∈ sb <-> in_supp b t) ->
+        is_derivable (sq_build (C +: foldr ty_arr T (type_check_other <$> sb)) ((
+          subst_last C (S C) (foldl tm_app (tm_lvl C) sb) b
+        ) :: (sq_set_map (lift C) l)) (lift C c)) ->
         is_derivable (sq_build C (<{ex T, b}> :: l) c)
     | rl_exR C T l b t :
         has_type C t T ->
-        is_derivable (sq_build C l (subst_last |(C)| t b)) ->
+        is_derivable (sq_build C l (subst_last C C t b)) ->
         is_derivable (sq_build C l <{ex T, b}>)
     | rl_nabL C T l b c n :
-        gtm_nom T n ∉ supp b ->
-        is_derivable (sq_build C (subst_last |(C)| (gtm_nom T n) b :: l) c) ->
+        ~ in_supp b (gtm_nom T n) ->
+        is_derivable (sq_build C (subst_last C C (gtm_nom T n) b :: l) c) ->
         is_derivable (sq_build C (<{nab T, b}> :: l) c)
     | rl_nabR C T l b n :
-        gtm_nom T n ∉ supp b ->
-        is_derivable (sq_build C l (subst_last |(C)| (gtm_nom T n) b)) ->
+        ~ in_supp b (gtm_nom T n) ->
+        is_derivable (sq_build C l (subst_last C C (gtm_nom T n) b)) ->
         is_derivable (sq_build C l (<{nab T, b}>))
   .
 
-  Theorem th C T h l t :
+
+  Theorem has_type_fold C T h l t :
     Forall2 (fun x X => has_type C x X) l h ->
     has_type C t (foldr ty_arr T h) ->
     has_type C (foldl tm_app t l) T.
   Proof.
-    generalize dependent t. generalize dependent h.
-    induction l; intros h t F Ht.
+    revert h t. induction l; intros h t F Ht.
     - inversion F. now subst.
     - simpl. destruct h; inversion F. subst.
       eapply IHl; try eassumption.
-      tm_simpl. exists t0. now split.
+      tm_simpl. now exists t0.
+  Qed.
+
+  Theorem has_type_fold2 C T sb b :
+    (forall t, t ∈ sb -> in_supp b t) ->
+    has_type (C +: foldr ty_arr T (type_check_other <$> sb)) (subst_last C (S C) (foldl tm_app (tm_lvl C) sb) b) -[ o ]- ->
+    has_type (C +: T) b ty_prp.
+  Proof.
+    intros.
+    eapply (has_type_subst_last2 _ (C +: foldr ty_arr T (type_check_other <$> sb)));
+      simpl; try eassumption; try lia.
+    - intros. now rewrite decide_True.
+    - eapply has_type_fold; tm_simpl; [|rewrite decide_False; intuition lia].
+      remember (C +: foldr ty_arr T (type_check_other <$> sb)) as D eqn : ED.
+      clear ED H0. induction sb; simpl in *; constructor.
+      + constructor. set_unfold. eapply in_supp_other. auto.
+      + set_unfold. auto.
   Qed.
 
   Theorem is_derivable_wf K : is_derivable K -> wf_sequent K.
@@ -140,130 +156,53 @@ Module GLogic (SqSet : SQ_SET).
     intros D. induction D; simpl in *.
     - split.
       + eapply has_type_tm_equiv; eassumption.
-      + intros t Ht.
-        apply elem_of_singleton in Ht. now subst.
-    - intuition. apply elem_of_union in H3 as [Ht | Ht]; [auto|].
-      + apply H2. apply elem_of_union. now left.
-    - intuition. apply H0. apply elem_of_union. now left.
-    - intuition. set_unfold. destruct H2; [auto|].
-      now subst.
-    - intuition. set_unfold. subst. now constructor.
-    - intuition.
-      + now constructor.
-      + now set_unfold.
-    - intuition. set_unfold. destruct H3.
-      + apply H0. intuition.
-      + subst. econstructor; [econstructor|]; intuition.
-        now apply ht_other2.
-    - intuition. econstructor; [econstructor|]; try eassumption.
-      now apply ht_other2.
-    - intuition. econstructor; [econstructor|]; try eassumption.
-      now apply ht_other2.
-    - intuition. set_unfold. destruct H2; [intuition|].
-      subst. econstructor; [econstructor|].
+      + intros. set_unfold. congruence.
+    - set_unfold. intuition.
+    - set_unfold. intuition.
+    - set_unfold. intuition. congruence.
+    - set_unfold. intuition. subst. now constructor.
+    - set_unfold. intuition. now constructor.
+    - set_unfold. intuition. subst.
+      repeat eapply ht_app; auto. now apply ht_other2.
+    - intuition. repeat eapply ht_app; try eassumption. now apply ht_other2.
+    - intuition. repeat eapply ht_app; try eassumption. now apply ht_other2.
+    - set_unfold. intuition. subst.
+      repeat eapply ht_app; eauto. now apply ht_other2.
+    - set_unfold. intuition. subst.
+      repeat eapply ht_app; eauto. now apply ht_other2.
+    - intuition. repeat eapply ht_app; try eassumption. now apply ht_other2.
+    - set_unfold. intuition. subst.
+      repeat eapply ht_app; eauto. now apply ht_other2.
+    - set_unfold. intuition.
+      repeat eapply ht_app; eauto. now apply ht_other2.
+    - set_unfold. intuition. subst. econstructor.
       + now apply ht_other2.
-      + apply H1. intuition.
-      + assumption.
-    - intuition. set_unfold. destruct H2; [intuition|].
-      subst. econstructor; [econstructor|].
-      + now apply ht_other2.
-      + assumption.
-      + apply H1. intuition.
-    - intuition. econstructor; [econstructor|]; try eassumption.
-      now apply ht_other2.
-    - intuition. set_unfold. destruct H3; intuition.
-      subst. econstructor; [econstructor|].
-      + now apply ht_other2.
-      + assumption.
-      + apply H2. intuition.
-    - intuition.
-      + econstructor; [econstructor|].
-        * now apply ht_other2.
-        * apply H0. set_unfold. intuition.
-        * assumption.
-      + apply H0. set_unfold. intuition.
-    - intuition. set_unfold. destruct H2.
-      + apply H1. intuition.
-      + subst. econstructor.
-        * now apply ht_other2.
-        * tm_simpl. exists ty_prp. split; [|reflexivity].
-          eapply has_type_subst_last; eauto.
+      + tm_simpl. eexists; try reflexivity.
+        eapply has_type_subst_last2; eauto.
     - intuition; [econstructor|].
       + now apply ht_other2.
-      + tm_simpl. exists ty_prp. intuition.
-        eapply (has_type_subst_last2_2 _ (C +: foldr ty_arr T (has_type_other <$> sb))).
-        4:{ rewrite rlength_rcons. eassumption. }
-        * now rewrite rlength_rcons.
-        * intros. now rewrite lookup_rcons_lt.
-        * clear D H0 H1.
-          eapply th.
-          2:{
-            tm_simpl. now rewrite @lookup_rcons_eq.
-          }
-          remember (C +: foldr ty_arr T (has_type_other <$> sb)) as D.
-          clear HeqD.
-          assert (forall t, t ∈ sb -> t ∈ supp b). { intros. now apply H. }
-          clear H.
-          induction sb.
-          -- simpl. constructor.
-          -- simpl in *. constructor.
-             ++ constructor. eapply supp_other. apply H0. set_unfold. intuition.
-             ++ apply IHsb. intros. apply H0. set_unfold. intuition.
-      + eapply (has_type_bound_level_map2 1).
-        3:{
-          specialize H1 with (bound_level_map S |(C)| t0).
-          unfold bound_level_map in *. erewrite level_map_f_eq.
-          - apply H1. apply sq_set_map_spec. exists t0. now split.
-          - simpl. now intros n.
-        }
-        * apply rlength_rcons.
-        * intros n Hn. now apply lookup_rcons_lt.
+      + tm_simpl. eexists; intuition.
+        eapply has_type_fold2; try eassumption. apply H.
+      + eapply has_type_lift2.
+        apply H1. apply sq_set_map_spec. eauto.
     - set_unfold. intuition.
-      + eapply (has_type_bound_level_map2 1); try eassumption.
-        * apply rlength_rcons.
-        * intros n Hn. now apply lookup_rcons_lt.
-      + eapply (has_type_bound_level_map2 1).
-        3:{
-          specialize H1 with (bound_level_map S |(C)| x).
-          unfold bound_level_map in *. erewrite level_map_f_eq.
-          - apply H1. left. apply sq_set_map_spec. exists x. intuition.
-          - intros. now simpl.
-        }
-        * apply rlength_rcons.
-        * intros n Hn. now apply lookup_rcons_lt.
+      + eapply has_type_lift2; eassumption.
+      + eapply has_type_lift2. apply H1. left.
+        apply sq_set_map_spec. eauto.
       + subst. econstructor; [now apply ht_other2|].
-        tm_simpl. exists ty_prp. intuition.
-        eapply (has_type_subst_last2_2 _ (C +: foldr ty_arr T (has_type_other <$> sb))).
-        4:{ rewrite rlength_rcons. apply H1. now right. }
-        * now rewrite rlength_rcons.
-        * intros. symmetry. now apply lookup_rcons_lt.
-        * clear D H0 H1.
-          eapply th.
-          2:{
-            tm_simpl. now rewrite @lookup_rcons_eq.
-          }
-          remember (C +: foldr ty_arr T (has_type_other <$> sb)) as D.
-          clear HeqD.
-          assert (forall t, t ∈ sb -> t ∈ supp b). { intros. now apply H. }
-          clear H.
-          induction sb.
-          -- simpl. constructor.
-          -- simpl in *. constructor.
-             ++ constructor. eapply supp_other. apply H0. set_unfold. intuition.
-             ++ apply IHsb. intros. apply H0. set_unfold. intuition.
+        tm_simpl. eexists; try reflexivity.
+        eapply has_type_fold2; auto. apply H.
     - intuition. econstructor; [now apply ht_other2|].
-      tm_simpl. exists ty_prp. split; [|easy].
-      eapply has_type_subst_last; eauto.
-    - intuition. set_unfold. destruct H2.
-      + apply H1. intuition.
-      + subst. econstructor; [now apply ht_other2|].
-        tm_simpl. eexists. split; [|reflexivity].
-        eapply has_type_subst_last.
-        2:{ apply H1. now right. }
-        now constructor.
+      tm_simpl. eexists; [|reflexivity].
+      eapply has_type_subst_last2; eauto.
+    - set_unfold. intuition. subst.
+      econstructor; [now apply ht_other2|].
+      tm_simpl. eexists; [|reflexivity].
+      eapply has_type_subst_last2; eauto.
+      now constructor.
     - intuition. econstructor; [now apply ht_other2|].
-      tm_simpl. eexists. split; [|reflexivity].
-      eapply has_type_subst_last; try eassumption.
+      tm_simpl. eexists; [|reflexivity].
+      eapply has_type_subst_last2; eauto.
       now constructor.
   Qed.
 End GLogic.
